Rework CoreExpr interpreter

src/CoreExpr/CEInterpreter.v
@@ -9,6 +9,9 @@ From Velus Require Import Environment.
 From Velus Require Import Operators.
 From Velus Require Import Clocks.
 From Velus Require Import CoreExpr.CESyntax.
+From Velus Require Import CoreExpr.CEIsFree.
+From Velus Require Import CoreExpr.CETyping.
+From Velus Require Import CoreExpr.CEClocking.
 From Velus Require Import CoreExpr.Stream.
 From Velus Require Import CoreExpr.CESemantics.
 
@@ -20,7 +23,10 @@ Module Type CEINTERPRETER
        (Import OpAux : OPERATORS_AUX   Op)
        (Import CESyn : CESYNTAX        Op)
        (Import Str   : STREAM          Op OpAux)
-       (Import CESem : CESEMANTICS Ids Op OpAux CESyn Str).
+       (Import CESem : CESEMANTICS Ids Op OpAux CESyn Str)
+       (Import CETyp : CETYPING    Ids Op       CESyn)
+       (Import CEClk : CECLOCKING  Ids Op       CESyn)
+       (Import CEFree: CEISFREE    Ids Op       CESyn).
 
   (** ** Instantaneous semantics *)
 
@@ -31,364 +37,888 @@ Module Type CEINTERPRETER
     Variable base : bool.
     Variable R: env.
 
-    Definition interp_var_instant (x: ident): value :=
-      match Env.find x R with
-      | Some v => v
-      | None => absent
-      end.
+    Definition interp_var_instant (x: ident): option value :=
+      Env.find x R.
 
-    Definition interp_vars_instant (xs: list ident): list value :=
-      map interp_var_instant xs.
+    (* TODO: Move elsewhere? *)
 
-    Fixpoint interp_clock_instant (c: clock): bool :=
+    Definition omap {A B : Type} (f : A -> option B) (xs : list A) : option (list B) :=
+      List.fold_right (fun x ys => match f x, ys with
+                                   | Some y, Some ys => Some (y :: ys)
+                                   | _, _ => None
+                                   end) (Some []) xs.
+
+    Definition interp_vars_instant (xs: list ident): option (list value) :=
+      omap interp_var_instant xs.
+
+    Fixpoint interp_clock_instant (c: clock) : option bool :=
       match c with
-      | Cbase =>
-        base
+      | Cbase => Some base
       | Con c x b =>
-        let cb := interp_clock_instant c in
-        match interp_var_instant x with
-        | present xv =>
-          match val_to_bool xv with
-          | Some b' =>
-            cb && b' ==b b
-          | None => false
-          end
-        | absent =>
-          false
+        match interp_clock_instant c with
+        | Some true => match interp_var_instant x with
+                       | Some (present xv) =>
+                         match val_to_bool xv with
+                         | Some xb => Some (xb ==b b)
+                         | None => None
+                         end
+                       | _ => None
+                       end
+        | Some false => match interp_var_instant x with
+                        | Some absent => Some false
+                        | _ => None
+                        end
+        | None => None
         end
       end.
 
-     Fixpoint interp_lexp_instant (e: lexp): value :=
-      match e with
-      | Econst c =>
-        if base then present (sem_const c) else absent
-      | Evar x _ =>
-        interp_var_instant x
-      | Ewhen e x b =>
-        match interp_var_instant x, interp_lexp_instant e with
-        | present xv, present ev =>
-          match val_to_bool xv with
-          | Some b' => if b ==b b' then present ev else absent
-          | None => absent
-          end
-        | _, _ => absent
-        end
-      | Eunop op e _ =>
-        match interp_lexp_instant e with
-        | present v =>
-          match sem_unop op v (typeof e) with
-          | Some v' => present v'
-          | None => absent
-          end
-        | absent => absent
-        end
-      | Ebinop op e1 e2 _ =>
-        match interp_lexp_instant e1, interp_lexp_instant e2 with
-        | present v1, present v2 =>
-          match sem_binop op v1 (typeof e1) v2 (typeof e2) with
-          | Some v => present v
-          | None => absent
-          end
-        | _, _ => absent
-        end
+     Fixpoint interp_lexp_instant (e: lexp) : option value :=
+       match e with
+       | Econst c => Some (if base then present (sem_const c) else absent)
+       | Evar x _ => interp_var_instant x
+       | Ewhen e x b =>
+           match interp_var_instant x, interp_lexp_instant e with
+           | Some (present xv), Some (present ev) =>
+               option_map (fun b'=> if b' ==b b then present ev else absent)
+                          (val_to_bool xv)
+           | Some absent, Some absent => Some absent
+           | _, _ => None
+           end
+       | Eunop op e _ =>
+           match interp_lexp_instant e with
+           | Some (present v) => option_map present (sem_unop op v (typeof e))
+           | vo => vo
+           end
+       | Ebinop op e1 e2 _ =>
+           match interp_lexp_instant e1, interp_lexp_instant e2 with
+           | Some (present v1), Some (present v2) =>
+               option_map present
+                          (sem_binop op v1 (typeof e1) v2 (typeof e2))
+           | Some absent, Some absent => Some absent
+           | _, _ => None
+           end
       end.
 
-    Definition interp_lexps_instant (les: list lexp): list value :=
-      map interp_lexp_instant les.
+    Definition interp_lexps_instant (les: list lexp) : option (list value) :=
+      omap interp_lexp_instant les.
 
-    Fixpoint interp_cexp_instant (e: cexp): value :=
+    Fixpoint interp_cexp_instant (e: cexp) : option value :=
       match e with
       | Emerge x t f =>
-        match interp_var_instant x, interp_cexp_instant t, interp_cexp_instant f with
-        | present xv, present tv, absent =>
-          if xv ==b true_val then present tv else absent
-        | present xv, absent, present fv =>
-          if xv ==b false_val then present fv else absent
-        | _, _, _ => absent
+        match interp_var_instant x with
+        | Some (present xv) =>
+          match val_to_bool xv, interp_cexp_instant t, interp_cexp_instant f with
+          | Some true, Some (present tv), Some absent => Some (present tv)
+          | Some false, Some absent, Some (present fv) => Some (present fv)
+          | _, _, _ => None
+          end
+        | Some absent =>
+          match interp_cexp_instant t, interp_cexp_instant f with
+          | Some absent, Some absent => Some absent
+          | _, _ => None
+          end
+        | None => None
         end
-
       | Eite b t f =>
         match interp_lexp_instant b, interp_cexp_instant t, interp_cexp_instant f with
-        | present bv, present tv, present fv =>
-          match val_to_bool bv with
-          | Some b' => present (if b' then tv else fv)
-          | None => absent
-          end
-        | _, _, _ => absent
+        | Some (present bv), Some (present tv), Some (present fv) =>
+          option_map (fun (b : bool) => if b then present tv else present fv)
+                     (val_to_bool bv)
+        | Some absent, Some absent, Some absent => Some absent
+        | _, _, _ => None
         end
-
-      | Eexp e =>
-        interp_lexp_instant e
+      | Eexp e => interp_lexp_instant e
       end.
 
-    Lemma interp_var_instant_sound:
+    Lemma interp_var_instant_correct:
       forall x v,
-        sem_var_instant R x v ->
-        v = interp_var_instant x.
-    Proof.
-      unfold interp_var_instant; now intros * ->.
-    Qed.
+        sem_var_instant R x v <-> interp_var_instant x = Some v.
+    Proof. reflexivity. Qed.
 
-    Ltac rw_lexp_helper :=
-      repeat match goal with
-             | _: sem_var_instant R ?x ?v |- context[interp_var_instant ?x] =>
-               erewrite <-(interp_var_instant_sound x v); eauto; simpl
-             | H: val_to_bool ?x = _ |- context[val_to_bool ?x] =>
-               rewrite H
-             | H: sem_unop ?op ?c ?t = _ |- context[sem_unop ?op ?c ?t] =>
-               rewrite H
-             | H: sem_binop ?op ?c1 ?t1 ?c2 ?t2 = _ |- context[sem_binop ?op ?c1 ?t1 ?c2 ?t2] =>
-               rewrite H
-          end.
-
-    Lemma interp_vars_instant_sound:
+    Lemma interp_vars_instant_correct:
       forall xs vs,
-        sem_vars_instant R xs vs ->
-        vs = interp_vars_instant xs.
+        sem_vars_instant R xs vs <-> interp_vars_instant xs = Some vs.
     Proof.
       unfold sem_vars_instant, interp_vars_instant.
-      induction 1; auto; simpl; rw_lexp_helper; f_equal; auto.
-    Qed.
+      induction xs as [|x xs IH]. now split; inversion 1.
+      destruct vs as [|v vs].
+      - split; intro HH. now inv HH.
+        simpl in HH.
+        destruct (interp_var_instant x); [|discriminate].
+        destruct (omap interp_var_instant xs); discriminate.
+      - split; intro HH.
+        + simpl. inversion_clear HH as [|???? Hsem FA2].
+          apply IH in FA2. rewrite FA2.
+          rewrite interp_var_instant_correct in Hsem. now rewrite Hsem.
+        + simpl in HH.
+          destruct (interp_var_instant x) eqn:Hsv; [|discriminate].
+          rewrite <-interp_var_instant_correct in Hsv.
+          destruct (omap interp_var_instant xs) eqn:Hxs; [|discriminate].
+          inv HH. constructor; auto.
+          now apply IH.
+    Qed.          
 
-    Lemma interp_clock_instant_sound:
+    (* TODO: move me *)
+    Lemma equiv_decb_negb:
+      forall x, (x ==b negb x) = false.
+    Proof. destruct x; simpl; auto. Qed.
+
+    Lemma interp_clock_instant_correct:
       forall c b,
-        sem_clock_instant base R c b ->
-        b = interp_clock_instant c.
+        sem_clock_instant base R c b <-> interp_clock_instant c = Some b.
     Proof.
-      induction 1; auto; simpl; rw_lexp_helper;
-        rewrite <-IHsem_clock_instant; destruct b; auto.
+      induction c as [|c IH].
+      now simpl; split; inversion 1; eauto using sem_clock_instant.
+      split; intro HH.
+      - inv HH; simpl;
+        repeat match goal with
+               | H:sem_clock_instant _ _ _ _ |- _ => apply IH in H; rewrite H
+               | H:sem_var_instant _ _ _ |- _ =>
+                 rewrite interp_var_instant_correct in H; rewrite H
+               | H:val_to_bool _ = _ |- _ =>
+                 rewrite H, ?equiv_decb_refl, ?equiv_decb_negb
+               end; auto.
+      - inv HH.
+        destruct (interp_clock_instant c) as [cb|] eqn:Hc; [|discriminate].
+        destruct (interp_var_instant i) eqn:Hi; [|destruct cb; discriminate].
+        apply interp_var_instant_correct in Hi.
+        destruct cb.
+        + destruct v as [|vc]; [discriminate|].
+          destruct (val_to_bool vc) as [vcb|] eqn:Hvc; [|discriminate].
+          match goal with H:Some _ = Some _ |- _ => inv H end.
+          destruct vcb, b; unfold equiv_decb; simpl.
+          * eapply Son; eauto; now apply IH.
+          * assert (false = negb true) as Hf by auto.
+            rewrite Hf at 1. eapply Son_abs2; eauto; now apply IH.
+          * assert (true = negb false) as Hf by auto.
+            rewrite Hf at 1. eapply Son_abs2; eauto; now apply IH.
+          * eapply Son; eauto; now apply IH.
+        + destruct v as [|vc]; [|discriminate].
+          match goal with H:Some _ = Some _ |- _ => inv H end.
+          eapply Son_abs1; auto. now apply IH.
     Qed.
 
-    Lemma interp_lexp_instant_sound:
+    Lemma interp_lexp_instant_correct:
       forall e v,
-        sem_lexp_instant base R e v ->
-        v = interp_lexp_instant e.
+        sem_lexp_instant base R e v <-> interp_lexp_instant e = Some v.
     Proof.
-      induction 1; simpl;
-        try rewrite <-IHsem_lexp_instant;
-        try rewrite <-IHsem_lexp_instant1;
-        try rewrite <-IHsem_lexp_instant2;
-        rw_lexp_helper; auto;
-          destruct b; auto.
+      induction e; simpl.
+      - (* Econst *)
+        split; inversion_clear 1; subst; eauto using sem_lexp_instant.
+      - (* Evar *)
+        setoid_rewrite <-interp_var_instant_correct.
+        split; [inversion_clear 1|]; eauto using sem_lexp_instant.
+      - (* Ewhen *)
+        split; intro HH.
+        + inv HH;
+          repeat match goal with
+                 | H:sem_var_instant _ _ _ |- _ =>
+                   rewrite interp_var_instant_correct in H; rewrite H
+                 | H:sem_lexp_instant _ _ _ _ |- _ =>
+                   rewrite IHe in H; rewrite H
+                 | H:val_to_bool _ = _ |- _ => rewrite H
+                 end; simpl; rewrite ?equiv_decb_refl, ?equiv_decb_negb; auto.
+        + destruct (interp_var_instant i) as [vi|] eqn:Hi; [|discriminate].
+          apply interp_var_instant_correct in Hi.
+          destruct (interp_lexp_instant e) as [ev|];
+            [|destruct vi; discriminate].
+          edestruct IHe as (N & IH); clear IHe N; specialize (IH eq_refl).
+          destruct vi.
+          now destruct ev; [inv HH; eauto using sem_lexp_instant|discriminate].
+          destruct ev as [|ev]; [discriminate|].
+          destruct (val_to_bool c) as [cb|] eqn:Hc; [|discriminate].
+          simpl in *.
+          destruct (cb ==b b) eqn:Hcb; inv HH;
+            rewrite ?equiv_decb_equiv in Hcb; rewrite ?Hcb in *;
+              eauto using sem_lexp_instant.
+          assert (b = negb cb) as ->
+              by (apply not_equiv_decb_equiv in Hcb;
+                  destruct b, cb; auto; exfalso; now apply Hcb).
+          eauto using sem_lexp_instant.
+      - (* Eunop *)
+        split; intro HH.
+        + inv HH; repeat match goal with
+                         | H:sem_lexp_instant _ _ _ _ |- _ =>
+                           rewrite IHe in H; rewrite H
+                         | H:sem_unop _ _ _ = _ |- _ => rewrite H
+                         end; auto.
+        + destruct (interp_lexp_instant e) as [ve|]; [|discriminate].
+          edestruct IHe as (N & IH); clear IHe N; specialize (IH eq_refl).
+          destruct ve.
+          now inv HH; eauto using sem_lexp_instant.
+          destruct (sem_unop u c (typeof e)) eqn:Hu; [|discriminate].
+          inv HH; eauto using sem_lexp_instant.
+      - (* Ebinop *)
+        split; intro HH.
+        + inv HH; repeat match goal with
+                         | H:sem_lexp_instant _ _ _ _ |- _ =>
+                           rewrite ?IHe1, ?IHe2 in H; rewrite H
+                         | H:sem_binop _ _ _ _ _ = _ |- _ => rewrite H
+                         end; auto.
+        + destruct (interp_lexp_instant e1) as [ve1|]; [|discriminate].
+          edestruct IHe1 as (N & IH1); clear N IHe1; specialize (IH1 eq_refl).
+          destruct (interp_lexp_instant e2) as [ve2|]; [|destruct ve1; discriminate].
+          edestruct IHe2 as (N & IH2); clear IHe2 N; specialize (IH2 eq_refl).
+          destruct ve1 as [|v1], ve2 as [|v2]; try discriminate.
+          now inv HH; eauto using sem_lexp_instant.
+          destruct (sem_binop b v1 (typeof e1) v2 (typeof e2)) eqn:Hu; [|discriminate].
+          inv HH; eauto using sem_lexp_instant.
     Qed.
 
-    Lemma interp_lexps_instant_sound:
+    Lemma omap_interp_correct:
+      forall {E V} sem interp,
+        (forall (e : E) (v : V), sem e v <-> interp e = Some v) ->
+        forall es vs,
+          Forall2 sem es vs <-> omap interp es = Some vs.
+    Proof.
+      intros E V sem interp Hcor.
+      induction es as [|e es IH]; simpl.
+      now split; inversion_clear 1; [auto|constructor].
+      split; intro HH.
+      - inv HH.
+        repeat match goal with
+               | H:Forall2 _ _ _ |- _ => apply IH in H; rewrite H
+               | H:sem _ _ |- _ => apply Hcor in H; rewrite H
+               end; auto.
+      - destruct (interp e) as [ev|] eqn:He; [|discriminate].
+        apply Hcor in He.
+        destruct (omap interp es) as [evs|]; [|discriminate].
+        edestruct IH as (N & IH'); clear IH N; specialize (IH' eq_refl).
+        inv HH; auto.
+    Qed.
+
+    Lemma interp_lexps_instant_correct:
       forall es vs,
-        sem_lexps_instant base R es vs ->
-        vs = interp_lexps_instant es.
+        sem_lexps_instant base R es vs <-> interp_lexps_instant es = Some vs.
     Proof.
-      induction 1; simpl; auto.
-      f_equal; auto.
-      now apply interp_lexp_instant_sound.
+      apply omap_interp_correct.
+      apply interp_lexp_instant_correct.
     Qed.
 
-    Ltac rw_cexp_helper :=
-      repeat (rw_lexp_helper;
-              repeat match goal with
-                     | _: sem_lexp_instant base R ?e ?v |- context[interp_lexp_instant ?e] =>
-                       erewrite <-(interp_lexp_instant_sound e v); eauto; simpl
-                     end).
-
-    Lemma interp_cexp_instant_sound:
+    Lemma interp_cexp_instant_correct:
       forall e v,
-        sem_cexp_instant base R e v ->
-        v = interp_cexp_instant e.
+        sem_cexp_instant base R e v <-> interp_cexp_instant e = Some v.
     Proof.
-      induction 1; simpl;
-        try rewrite <-IHsem_cexp_instant;
-        try rewrite <-IHsem_cexp_instant1;
-        try rewrite <-IHsem_cexp_instant2;
-        rw_cexp_helper;
-        try rewrite equiv_decb_refl; auto;
-          destruct b; auto.
+      induction e.
+      - (* Emerge *)
+        split; intro HH.
+        + inv HH; simpl;
+            repeat match goal with
+                   | H:sem_var_instant _ _ _ |- _ =>
+                     rewrite interp_var_instant_correct in H; rewrite H
+                   | H:sem_cexp_instant _ _ _ _ |- _ =>
+                     rewrite ?IHe1, ?IHe2 in H; rewrite H
+                   end;
+            now rewrite ?val_to_bool_true, ?val_to_bool_false.
+        + simpl in HH.
+          destruct (interp_var_instant i) as [iv|] eqn:Hi; [|discriminate].
+          destruct iv.
+          * destruct (interp_cexp_instant e1) as [v1|]; [|discriminate].
+            destruct v1; [|discriminate].
+            destruct (interp_cexp_instant e2) as [v2|]; [|discriminate].
+            destruct v2; [|discriminate].
+            edestruct IHe1 as (N & IH1); clear IHe1 N; specialize (IH1 eq_refl).
+            edestruct IHe2 as (N & IH2); clear IHe2 N; specialize (IH2 eq_refl).
+            inv HH; eauto using sem_cexp_instant.
+          * destruct (interp_cexp_instant e1) as [v1|] eqn:He1;
+              destruct (val_to_bool c) eqn:Hc;
+              try destruct b;
+              try discriminate;
+              try apply val_to_bool_true' in Hc;
+              try apply val_to_bool_false' in Hc;
+              (edestruct IHe1 as (N & IH1); clear IHe1 N; specialize (IH1 eq_refl));
+              destruct (interp_cexp_instant e2) as [v2|] eqn:He2;
+              try (edestruct IHe2 as (N & IH2); clear IHe2 N; specialize (IH2 eq_refl));
+              subst;
+              try destruct v1;
+              try destruct v2;
+              try discriminate;
+              inv HH; eauto using sem_cexp_instant.
+      - (* Eite *)
+        split; intro HH.
+        + inv HH; simpl;
+            repeat match goal with
+                   | H:sem_lexp_instant _ _ _ _ |- _ =>
+                     rewrite interp_lexp_instant_correct in H; rewrite H
+                   | H:sem_cexp_instant _ _ _ _ |- _ =>
+                     rewrite ?IHe1, ?IHe2 in H; rewrite H
+                   | H:val_to_bool _ = _ |- _ => rewrite H
+                   end; try destruct b; auto.
+        + simpl in HH.
+          destruct (interp_lexp_instant l) as [iv|] eqn:Hi; [|discriminate].
+          apply interp_lexp_instant_correct in Hi.
+          destruct (interp_cexp_instant e1) as [v1|]; [|destruct iv; discriminate].
+          destruct (interp_cexp_instant e2) as [v2|]; [|destruct iv, v1; discriminate].
+          edestruct IHe1 as (N & IH1); clear IHe1 N; specialize (IH1 eq_refl).
+          edestruct IHe2 as (N & IH2); clear IHe2 N; specialize (IH2 eq_refl).
+          destruct iv; destruct v1, v2; try discriminate.
+          now inv HH; eauto using sem_cexp_instant.
+          destruct (val_to_bool c) eqn:Hc; [|discriminate].
+          inv HH; eauto using sem_cexp_instant.
+      - (* Eexp *)
+        simpl. setoid_rewrite <-interp_lexp_instant_correct.
+        split; intro HH; [now inv HH|now constructor].
     Qed.
 
-    Definition interp_annotated_instant {A} (interp: A -> value) (ck: clock) (a: A): value :=
-      if interp_clock_instant ck then
-        interp a
-      else
-        absent.
+    Definition interp_annotated_instant {E} (interp : E -> option value)
+               (ck : clock) (e : E) : option value :=
+      match interp_clock_instant ck, interp e with
+      | Some true, Some (present v) => Some (present v)
+      | Some false, Some absent => Some absent
+      | _, _ => None
+      end.
 
-    Definition interp_caexp_instant (ck: clock) (ce: cexp) : value :=
-      interp_annotated_instant (interp_cexp_instant) ck ce.
+    Definition interp_laexp_instant ck e :=
+      interp_annotated_instant interp_lexp_instant ck e.
 
-    Lemma interp_caexp_instant_sound:
+    Definition interp_caexp_instant ck e :=
+      interp_annotated_instant interp_cexp_instant ck e.
+
+    Lemma interp_laexp_instant_correct:
       forall ck e v,
-        sem_caexp_instant base R ck e v ->
-        v = interp_caexp_instant ck e.
-    Proof.
-      unfold interp_caexp_instant, interp_annotated_instant.
-      induction 1; erewrite <-interp_clock_instant_sound; eauto; simpl; auto.
-      apply interp_cexp_instant_sound; auto.
-    Qed.
-
-    Definition interp_laexp_instant (ck: clock) (e: lexp) : value :=
-      interp_annotated_instant (interp_lexp_instant) ck e.
-
-    Lemma interp_laexp_instant_sound:
-      forall ck e v,
-        sem_laexp_instant base R ck e v ->
-        v = interp_laexp_instant ck e.
+        sem_laexp_instant base R ck e v <-> interp_laexp_instant ck e = Some v.
     Proof.
       unfold interp_laexp_instant, interp_annotated_instant.
-      induction 1; erewrite <-interp_clock_instant_sound; eauto; simpl; auto.
-      apply interp_lexp_instant_sound; auto.
+      split; intro HH.
+      - inversion_clear HH as [??? Hs Hck|?? Hs Hck];
+          apply interp_lexp_instant_correct in Hs as ->;
+          now apply interp_clock_instant_correct in Hck as ->.
+      - destruct (interp_clock_instant ck) eqn:Hck;
+          try apply interp_clock_instant_correct in Hck;
+          destruct (interp_lexp_instant e) as [ev|] eqn:He;
+          try apply interp_lexp_instant_correct in He;
+          try destruct b;
+          try destruct ev;
+          try discriminate;
+          inv HH; now constructor.
+    Qed.
+
+    Lemma interp_caexp_instant_correct:
+      forall ck e v,
+        sem_caexp_instant base R ck e v <-> interp_caexp_instant ck e = Some v.
+    Proof.
+      unfold interp_caexp_instant, interp_annotated_instant.
+      split; intro HH.
+      - inversion_clear HH as [??? Hs Hck|?? Hs Hck];
+          apply interp_cexp_instant_correct in Hs as ->;
+          now apply interp_clock_instant_correct in Hck as ->.
+      - destruct (interp_clock_instant ck) eqn:Hck;
+          try apply interp_clock_instant_correct in Hck;
+          destruct (interp_cexp_instant e) as [ev|] eqn:He;
+          try apply interp_cexp_instant_correct in He;
+          try destruct b;
+          try destruct ev;
+          try discriminate;
+          inv HH; now constructor.
+    Qed.
+
+    (** Existence proofs *)
+    
+    Variable vars : list (ident * (type * clock)).
+    Hypothesis NDvars : NoDupMembers vars.
+
+    Inductive Ops_defined_in_lexp : lexp -> Prop :=
+    | ODconst : forall c,
+        Ops_defined_in_lexp (Econst c)
+    | ODvar: forall x ty,
+        Ops_defined_in_lexp (Evar x ty)
+    | ODwhen : forall e x b,
+        Ops_defined_in_lexp e ->
+        Ops_defined_in_lexp (Ewhen e x b)
+    | ODunop : forall op e ty,
+        Ops_defined_in_lexp e ->
+        (forall v, sem_lexp_instant base R e (present v) ->
+                   sem_unop op v (typeof e) <> None) ->        
+        Ops_defined_in_lexp (Eunop op e ty)
+    | ODbinop: forall op e1 e2 ty,
+        Ops_defined_in_lexp e1 ->
+        Ops_defined_in_lexp e2 ->
+        (forall v1 v2,
+            sem_lexp_instant base R e1 (present v1) ->
+            sem_lexp_instant base R e2 (present v2) ->
+            sem_binop op v1 (typeof e1) v2 (typeof e2) <> None) ->
+        Ops_defined_in_lexp (Ebinop op e1 e2 ty).
+
+    Inductive Ops_defined_in_cexp : cexp -> Prop :=
+    | ODmerge : forall x et ef,
+        Ops_defined_in_cexp et ->
+        Ops_defined_in_cexp ef ->
+        Ops_defined_in_cexp (Emerge x et ef)
+    | ODite : forall e et ef,
+        Ops_defined_in_lexp e ->
+        Ops_defined_in_cexp et ->
+        Ops_defined_in_cexp ef ->
+        Ops_defined_in_cexp (Eite e et ef)
+    | ODexp : forall e,
+        Ops_defined_in_lexp e ->
+        Ops_defined_in_cexp (Eexp e).
+
+    Definition var_inv (D : positive -> Prop) : Prop :=
+      forall x, D x ->
+                exists xv, sem_var_instant R x xv
+                           /\ (exists xt xc cs,
+                                  In (x, (xt, xc)) vars
+                                  /\ sem_clock_instant base R xc cs
+                                  /\ match xv with
+                                     | absent => cs = false
+                                     | present v => cs = true /\ wt_val v xt
+                                     end).
+
+    Lemma var_inv_weaken:
+      forall (D1 D2 : positive -> Prop),
+        var_inv D1 ->
+        (forall x, D2 x -> D1 x) ->
+        var_inv D2.
+    Proof.
+      intros D1 D2 I1 H12 x D2x.
+      now apply H12, I1 in D2x.
+    Qed.
+
+    Local Ltac tidy_wt_wc :=
+      repeat match goal with
+             | H:In _ (idck vars) |- _ =>
+               apply In_idck_exists in H as (xt' & I1'); clear H
+             | H:In _ (idty vars) |- _ =>
+               apply In_idty_exists in H as (xc' & I2'); clear H
+             | H1:In (?x1, (?t1, ?c1)) vars, H2:In (?x2, (?t2, ?c2)) vars |- _ =>
+               apply (NoDupMembers_det _ _ _ _ NDvars H1) in H2; inv H2
+             end.
+
+    (* TODO: Generalize and move to CESemantics? *)
+    Local Ltac sem_det :=
+      repeat match goal with
+             | H1:sem_var_instant _ _ _, H2:sem_var_instant _ _ _ |- _ =>
+               apply (sem_var_instant_det _ _ _ _ H1) in H2; subst
+             | H1:sem_clock_instant _ _ _ _, H2:sem_clock_instant _ _ _ _ |- _ =>
+               apply (sem_clock_instant_det _ _ _ _ _ H1) in H2; subst
+             | H:present _ = present _ |- _ => inv H
+             | H1:val_to_bool ?x = _, H2:val_to_bool ?x = _ |- _ =>
+               rewrite H1 in H2; inv H2
+             end.
+
+    (* Exploit hypotheses of the forms: absent = absent <-> cks = false,
+       present c = absent <-> cks = false, etc. *)      
+    Local Ltac break_status_cks_iffs :=
+      assert (forall v, present v <> absent) as Hpa by discriminate;
+      repeat match goal with
+             | H:?x = ?x <-> ?cks = ?b |- _ =>
+               destruct H as (H & ?); specialize (H eq_refl)
+             | H:present ?c = absent <-> ?cks = ?b |- _ =>
+               apply not_iff_compat in H;
+               rewrite Bool.not_false_iff_true in H;
+               destruct H as (H & ?);
+               specialize (H (Hpa _))
+             | H:?x = ?x -> _ |- _ => specialize (H eq_refl)
+             end; clear Hpa; subst.
+
+    Lemma interp_clock_instant_good:
+      forall ck,
+        wt_clock (idty vars) ck ->
+        wc_clock (idck vars) ck ->
+        var_inv (fun x => Is_free_in_clock x ck) ->
+        exists v, interp_clock_instant ck = Some v.
+    Proof.
+      induction ck as [|ck IH x]. now simpl; eauto.
+      intros WT WC Inv.
+      inv WT. inv WC.
+      match goal with WT:wt_clock _ _, WC:wc_clock _ _ |- _ =>
+                      specialize (IH WT WC) as (v & Hck) end.
+      now eapply var_inv_weaken; [eassumption|simpl; auto].
+      specialize (Inv x (FreeCon1 x _ _)) as (xv & Sx & (xt & xc & cs & I1 & I2 & I3)).
+      simpl. setoid_rewrite Hck.
+      tidy_wt_wc.
+      apply interp_clock_instant_correct in I2.
+      rewrite Hck in I2; inv I2.
+      rewrite interp_var_instant_correct in Sx; rewrite Sx.
+      destruct xv; [|destruct I3 as (Hcs & WTv)]; subst; eauto.
+      apply wt_val_to_bool in WTv as (cb & WTv). rewrite WTv; eauto.
+    Qed.
+
+    Corollary sem_clock_instant_good:
+      forall ck,
+        wt_clock (idty vars) ck ->
+        wc_clock (idck vars) ck ->
+        var_inv (fun x => Is_free_in_clock x ck) ->
+        exists v, sem_clock_instant base R ck v.
+    Proof.
+      setoid_rewrite interp_clock_instant_correct.
+      auto using interp_clock_instant_good.
+    Qed.
+
+    Lemma sem_lexp_instant_clocked:
+      forall e ck v,
+        wc_lexp (idck vars) e ck ->
+        var_inv (fun x => Is_free_in_lexp x e) ->
+        sem_lexp_instant base R e v ->
+        exists cks, sem_clock_instant base R ck cks
+                    /\ (v = absent <-> cks = false).
+    Proof.
+      induction e; simpl; intros ck v WC Inv Se; inv WC.
+      - (* Econst *)
+        inv Se. exists base.
+        split; eauto using sem_clock_instant.
+        destruct base; intuition; discriminate.
+      - (* Evar *)
+        specialize (Inv i (FreeEvar i _))
+          as (iv & Si & (it & ic & ics & I1 & I2 & I3)).
+        inv Se. tidy_wt_wc. sem_det.
+        exists ics. split; auto.
+        destruct v; intuition; subst; try discriminate.
+      - (* Ewhen *)
+        inv Se; sem_det; try discriminate;
+        repeat match goal with
+               | H:sem_lexp_instant _ _ _ _, WC:wc_lexp _ e _ |- _ =>
+                 eapply IHe with (1:=WC) in H as (cks & Scks & H); clear IHe
+               | |- var_inv _ =>
+                 now eapply var_inv_weaken; eauto; simpl; auto
+               end; break_status_cks_iffs;
+          eexists; (split; [eauto using sem_clock_instant|now intuition]).
+      - (* Eunop *)
+        assert (var_inv (fun x => Is_free_in_lexp x e)) as Inv'
+          by (apply (var_inv_weaken _ _ Inv); auto).
+        inv Se; match goal with
+                | WC:wc_lexp _ _ _, H:sem_lexp_instant _ _ _ _ |- _ =>
+                  specialize (IHe _ _ WC Inv' H)
+                end; destruct IHe as (cks & Scks & H); break_status_cks_iffs;
+          eexists; (split; [eauto using sem_clock_instant|now intuition]).
+      - (* Ebinop *)
+        assert (var_inv (fun x => Is_free_in_lexp x e1)) as Inv1
+          by (apply (var_inv_weaken _ _ Inv); auto).
+        assert (var_inv (fun x => Is_free_in_lexp x e2)) as Inv2
+          by (apply (var_inv_weaken _ _ Inv); auto).
+        inv Se; match goal with
+                  WC:wc_lexp _ _ _, H:sem_lexp_instant _ _ _ _ |- _ =>
+                  specialize (IHe1 _ _ WC Inv1 H) end;
+        destruct IHe1 as (cks1 & Scks1 & H1);
+        break_status_cks_iffs;
+        eexists; (split; [eauto using sem_clock_instant|now intuition]).
+    Qed.
+      
+    Lemma interp_lexp_instant_good:
+      forall e ck,
+        wt_lexp (idty vars) e ->
+        wc_lexp (idck vars) e ck ->
+        Ops_defined_in_lexp e ->
+        var_inv (fun x => Is_free_in_lexp x e) ->
+        exists v, interp_lexp_instant e = Some v.
+    Proof.
+      induction e; simpl; intros ck WT WC OD Inv.
+      - (* Econst *) eauto.
+      - (* Evar *)
+        specialize (Inv i (FreeEvar i _)) as (v & Hsem & Inv).
+        rewrite interp_var_instant_correct in Hsem. now eauto.
+      - (* Ewhen *)
+        inv WT. inv WC. inv OD.
+        match goal with
+          WT:wt_lexp _ _, WC:wc_lexp _ _ _, OD:Ops_defined_in_lexp _ |- _ =>
+          specialize (IHe _ WT WC OD) as (ev & Hv) end.
+        now eapply var_inv_weaken; [eassumption|simpl; auto].
+        rewrite Hv.
+        pose proof (Inv i (FreeEwhen2 _ i _))
+          as (iv & Si & (it & ic & ics & I1 & I2 & I3)).
+        tidy_wt_wc.
+        rewrite interp_var_instant_correct in Si; rewrite Si.
+        apply interp_lexp_instant_correct in Hv.
+        eapply sem_lexp_instant_clocked in Hv as (cks & Hs & H); eauto.
+        2:now eapply var_inv_weaken; [eassumption|simpl; auto].
+        sem_det. destruct iv.
+        + assert (ev = absent) by intuition. subst; eauto.
+        + destruct I3 as (? & WT).
+          assert (ev <> absent) as Habs by (subst; intuition).
+          apply not_absent_present in Habs as (v & ->).
+          apply wt_val_to_bool in WT as (? & ->). simpl; eauto.
+      - (* Eunop *)
+        inv WT. inv WC. inversion OD as [| | |??? ODe ODv|]; subst.
+        match goal with WT:wt_lexp _ _, WC:wc_lexp _ _ _ |- _ =>
+          specialize (IHe _ WT WC ODe) as (ev & Hv) end.
+        now eapply var_inv_weaken; [eassumption|simpl; auto].
+        rewrite Hv.
+        apply interp_lexp_instant_correct in Hv.
+        destruct ev; eauto.
+        apply ODv, not_None_is_Some in Hv as (v & ->); simpl; eauto.
+      - (* Ebinop *)
+        inv WT. inversion WC as [| | | |????? WC1 WC2].
+        inversion OD as [| | | |???? ODe1 ODe2 ODv]; subst.
+        repeat match goal with WT:wt_lexp _ _, WC:wc_lexp _ _ _ |- _ =>
+          specialize (IHe1 _ WT WC ODe1) as (ev1 & Hv1)
+          || specialize (IHe2 _ WT WC ODe2) as (ev2 & Hv2) end;
+          try (now eapply var_inv_weaken; [eassumption|simpl; auto]).
+        rewrite Hv1, Hv2.
+        apply interp_lexp_instant_correct in Hv1.
+        apply interp_lexp_instant_correct in Hv2.
+          eapply sem_lexp_instant_clocked in WC1 as (cks1 & Hs1 & HH1); eauto;
+            [|now eapply var_inv_weaken; [eassumption|simpl; auto]];
+          eapply sem_lexp_instant_clocked in WC2 as (cks2 & Hs2 & HH2); eauto;
+            [|now eapply var_inv_weaken; [eassumption|simpl; auto]];
+          sem_det.
+        destruct ev1, ev2; eauto; break_status_cks_iffs; try discriminate.
+        specialize (ODv _ _ Hv1 Hv2).
+        apply not_None_is_Some in ODv as (v & ->).
+        simpl; eauto.
+    Qed.
+
+    Corollary sem_lexp_instant_good:
+      forall e ck,
+        wt_lexp (idty vars) e ->
+        wc_lexp (idck vars) e ck ->
+        Ops_defined_in_lexp e ->
+        var_inv (fun x => Is_free_in_lexp x e) ->
+        exists v, sem_lexp_instant base R e v.
+    Proof.
+      setoid_rewrite interp_lexp_instant_correct.
+      eauto using interp_lexp_instant_good.
+    Qed.
+
+    Lemma sem_cexp_instant_clocked:
+      forall e ck v,
+        wc_cexp (idck vars) e ck ->
+        var_inv (fun x => Is_free_in_cexp x e) ->
+        sem_cexp_instant base R e v ->
+        exists cks, sem_clock_instant base R ck cks
+                    /\ (v = absent <-> cks = false).
+    Proof.
+      induction e; simpl; intros ck v WC Inv Se;
+        inversion WC as [???? Hin WC1 WC2|???? WCe WC1 WC2|?? WCe]; subst.
+      - (* Emerge *)
+        assert (var_inv (fun x=>Is_free_in_cexp x e1)) as Inv1
+            by (eapply var_inv_weaken; [eauto|simpl; intuition]).
+        assert (var_inv (fun x=>Is_free_in_cexp x e2)) as Inv2
+            by (eapply var_inv_weaken with (1:=Inv); intuition).
+        inv Se;
+        repeat match goal with Se:sem_cexp_instant _ _ _ _ |- _ =>
+          specialize (IHe1 _ _ WC1 Inv1 Se) as (cks1 & Sck1 & HH1)
+                                               || specialize (IHe2 _ _ WC2 Inv2 Se) as (cks2 & Sck2 & HH2) end;
+        break_status_cks_iffs.
+        + inv Sck1. eexists; split; [eauto|now intuition].
+          match goal with H1:negb _ = true, H2:false = negb _ |- _ =>
+            rewrite H1 in H2; discriminate end.
+        + inv Sck2. eexists; split; [eauto|now intuition].
+          match goal with H1:negb _ = true, H2:negb _ = false |- _ =>
+            rewrite H1 in H2; discriminate end.
+        + inv Sck1.
+          now eexists; split; [eauto|intuition].
+          eexists false; split; [sem_det;discriminate|now intuition].
+      - (* Eite *)
+        assert (var_inv (fun x=>Is_free_in_cexp x e1)) as Inv1
+            by (eapply var_inv_weaken; [eauto|simpl; intuition]).
+        assert (var_inv (fun x=>Is_free_in_cexp x e2)) as Inv2
+            by (eapply var_inv_weaken with (1:=Inv); intuition).
+        inv Se;
+        repeat match goal with Se:sem_cexp_instant _ _ _ _ |- _ =>
+          specialize (IHe1 _ _ WC1 Inv1 Se) as (cks1 & Sck1 & HH1)
+          || specialize (IHe2 _ _ WC2 Inv2 Se) as (cks2 & Sck2 & HH2) end;
+        break_status_cks_iffs; eexists; split; eauto; try destruct b; intuition.
+      - (* Eexp *)
+        inversion_clear Se as [| | | | |?? He].
+        apply (sem_lexp_instant_clocked _ _ _ WCe) in He as (cks & He & HH); eauto.
+        now eapply var_inv_weaken with (1:=Inv); intuition.
+    Qed.
+
+    Lemma sem_lexp_instant_wt_val:
+      forall e v,
+        sem_lexp_instant base R e (present v) ->
+        wt_lexp (idty vars) e ->
+        var_inv (fun x => Is_free_in_lexp x e) ->
+        wt_val v (typeof e).
+    Proof.
+      induction e; intros v Sv WT Inv.
+      - (* Econst *)
+        inv Sv. destruct base; [|discriminate].
+        match goal with H:present _ = present _ |- _ => inv H end.
+        apply wt_val_const.
+      - (* Evar *)
+        specialize (Inv i (FreeEvar i _))
+          as (iv & Si & (it & ic & ics & I1 & I2 & I3)).
+        inv Sv. sem_det. destruct I3 as (Hics & WTV).
+        inv WT. now tidy_wt_wc.
+      - (* Ewhen *)
+        inv Sv. inv WT. apply IHe; auto.
+        eapply var_inv_weaken; [eauto|now intuition].
+      - (* Eunop *)
+        inv Sv. inv WT. simpl.
+        eapply pres_sem_unop; eauto.
+        apply IHe; auto.
+        eapply var_inv_weaken; [eauto|now intuition].
+      - (* Ebinop *)
+        inv Sv. inv WT. simpl.
+        eapply pres_sem_binop; eauto.
+        now apply IHe1; auto; eapply var_inv_weaken; [eauto|intuition].
+        now apply IHe2; auto; eapply var_inv_weaken; [eauto|intuition].
+    Qed.
+
+    Lemma interp_cexp_instant_good:
+      forall e ck,
+        wt_cexp (idty vars) e ->
+        wc_cexp (idck vars) e ck ->
+        Ops_defined_in_cexp e ->
+        var_inv (fun x => Is_free_in_cexp x e) ->
+        exists v, interp_cexp_instant e = Some v.
+    Proof.
+      induction e; simpl; intros ck WT WC OD Inv;
+        inversion_clear WT as [????? WT1 WT2|???? WTe WT1 WT2|? WTe];
+        inversion_clear WC as [????? WC1 WC2|???? WCe WC1 WC2|?? WCe];
+        inversion_clear OD as [??? ODe1 ODe2|??? ODe ODe1 ODe2|? ODe].
+      - (* Emerge *)
+        epose proof (var_inv_weaken _ (fun x=>Is_free_in_cexp x e1) Inv _) as Inv1.
+        Unshelve. 2:now intuition.
+        epose proof (var_inv_weaken _ (fun x=>Is_free_in_cexp x e2) Inv _) as Inv2.
+        Unshelve. 2:now intuition.
+        specialize (IHe1 _ WT1 WC1 ODe1 Inv1) as (v1 & IHe1).
+        specialize (IHe2 _ WT2 WC2 ODe2 Inv2) as (v2 & IHe2).
+        rewrite IHe1, IHe2.
+        apply interp_cexp_instant_correct in IHe1.
+        apply interp_cexp_instant_correct in IHe2.
+        pose proof (Inv i (FreeEmerge_cond i _ _))
+          as (iv & Si & (it & ic & ics & I1 & I2 & I3)).
+        assert (Ii := Si). apply interp_var_instant_correct in Ii as ->.
+        apply (sem_cexp_instant_clocked _ _ _ WC1 Inv1) in IHe1
+          as (cks1 & Hck1 & HH1).
+        apply (sem_cexp_instant_clocked _ _ _ WC2 Inv2) in IHe2
+          as (cks2 & Hck2 & HH2).
+        inv Hck1; inv Hck2; destruct iv, v1, v2; subst; eauto;
+          break_status_cks_iffs;
+          repeat match goal with H:_ /\ _ |- _ => destruct H end;
+          subst; sem_det; try discriminate;
+          repeat match goal with
+                 | H:val_to_bool _ = _ |- _ => setoid_rewrite H; clear H
+                 | Ht:negb _ = true, Hf:negb _ = false |- _ => rewrite Ht in Hf
+                 end; eauto; discriminate.
+      - (* Eite *)
+        epose proof (var_inv_weaken _ (fun x=>Is_free_in_lexp x l) Inv _) as Inve.
+        Unshelve. 2:now intuition.
+        epose proof (var_inv_weaken _ (fun x=>Is_free_in_cexp x e1) Inv _) as Inv1.
+        Unshelve. 2:now intuition.
+        epose proof (var_inv_weaken _ (fun x=>Is_free_in_cexp x e2) Inv _) as Inv2.
+        Unshelve. 2:now intuition.
+        specialize (IHe1 _ WT1 WC1 ODe1 Inv1) as (v1 & IHe1).
+        specialize (IHe2 _ WT2 WC2 ODe2 Inv2) as (v2 & IHe2).
+        rewrite IHe1, IHe2.
+        apply interp_cexp_instant_correct in IHe1.
+        apply interp_cexp_instant_correct in IHe2.
+        pose proof (interp_lexp_instant_good _ _ WTe WCe ODe Inve) as (v & He).
+        rewrite He; apply interp_lexp_instant_correct in He.
+        pose proof (sem_lexp_instant_clocked _ _ _ WCe Inve He) as (cks & Hck & HH).
+        eapply sem_cexp_instant_clocked in IHe1 as (cks1 & Hck1 & HH1); eauto.
+        eapply sem_cexp_instant_clocked in IHe2 as (cks2 & Hck2 & HH2); eauto.
+        sem_det.
+        destruct v; break_status_cks_iffs.
+        + assert (v1 = absent) by intuition.
+          assert (v2 = absent) by intuition.
+          subst; eauto.
+        + assert (v1 <> absent) as Hv1 by intuition.
+          assert (v2 <> absent) as Hv2 by intuition.
+          apply not_absent_present in Hv1 as (c1 & Hc1).
+          apply not_absent_present in Hv2 as (c2 & Hc2).
+          subst. apply sem_lexp_instant_wt_val in He; auto. rewrite H in He.
+          apply wt_val_to_bool in He as (b & ->).
+          destruct b; simpl; eauto.
+      - (* Eexp *)
+        eapply interp_lexp_instant_good; eauto.
+        eapply var_inv_weaken; [eauto|now intuition].
+    Qed.
+
+    Corollary sem_cexp_instant_good:
+      forall e ck,
+        wt_cexp (idty vars) e ->
+        wc_cexp (idck vars) e ck ->
+        Ops_defined_in_cexp e ->
+        var_inv (fun x => Is_free_in_cexp x e) ->
+        exists v, sem_cexp_instant base R e v.
+    Proof.
+      setoid_rewrite interp_cexp_instant_correct.
+      eauto using interp_cexp_instant_good.
+    Qed.
+
+    Lemma sem_cexp_instant_wt_val:
+      forall e v,
+        sem_cexp_instant base R e (present v) ->
+        wt_cexp (idty vars) e ->
+        var_inv (fun x => Is_free_in_cexp x e) ->
+        wt_val v (typeofc e).
+    Proof.
+      induction e; intros v Sv WT Inv; simpl; inv WT.
+      - (* Emerge *)
+        inv Sv.
+        now apply IHe1; auto; eapply var_inv_weaken; [eauto|intuition].
+        match goal with H:typeofc _ = typeofc _ |- _ => rewrite H end.
+        now apply IHe2; auto; eapply var_inv_weaken; [eauto|intuition].
+      - (* Eite *)
+        inv Sv.
+        destruct b; match goal with H:present _ = present _ |- _ => inv H end.
+        now apply IHe1; auto; eapply var_inv_weaken; [eauto|intuition].
+        match goal with H:typeofc _ = typeofc _ |- _ => rewrite H end.
+        now apply IHe2; auto; eapply var_inv_weaken; [eauto|intuition].
+      - (* Eexp *)
+        inv Sv. apply sem_lexp_instant_wt_val; auto.
+        now eapply var_inv_weaken; [eauto|intuition].
+    Qed.
+
+    Lemma interp_laexp_instant_good:
+      forall e ck,
+        wt_lexp (idty vars) e ->
+        wt_clock (idty vars) ck ->
+        wc_lexp (idck vars) e ck ->
+        wc_clock (idck vars )ck ->
+        Ops_defined_in_lexp e ->
+        var_inv (fun x => Is_free_in_lexp x e) ->
+        var_inv (fun x => Is_free_in_clock x ck) ->
+        exists v, interp_laexp_instant ck e = Some v.
+    Proof.
+      intros e ck WT WTc WC WCc OD Inv Invc.
+      pose proof (interp_lexp_instant_good _ _ WT WC OD Inv) as (v & Iexp).
+      unfold interp_laexp_instant, interp_annotated_instant.
+      rewrite Iexp.
+      apply interp_lexp_instant_correct in Iexp.
+      eapply sem_lexp_instant_clocked in Iexp as (cks & Iclk & HH); eauto.
+      apply interp_clock_instant_correct in Iclk as ->.
+      destruct v; break_status_cks_iffs; eauto.
+    Qed.
+
+    Lemma interp_caexp_instant_good:
+      forall e ck,
+        wt_cexp (idty vars) e ->
+        wt_clock (idty vars) ck ->
+        wc_cexp (idck vars) e ck ->
+        wc_clock (idck vars )ck ->
+        Ops_defined_in_cexp e ->
+        var_inv (fun x => Is_free_in_cexp x e) ->
+        var_inv (fun x => Is_free_in_clock x ck) ->
+        exists v, interp_caexp_instant ck e = Some v.
+    Proof.
+      intros e ck WT WTc WC WCc OD Inv Invc.
+      pose proof (interp_cexp_instant_good _ _ WT WC OD Inv) as (v & Iexp).
+      unfold interp_caexp_instant, interp_annotated_instant.
+      rewrite Iexp.
+      apply interp_cexp_instant_correct in Iexp.
+      eapply sem_cexp_instant_clocked in Iexp as (cks & Iclk & HH); eauto.
+      apply interp_clock_instant_correct in Iclk as ->.
+      destruct v; break_status_cks_iffs; eauto.
+    Qed.
+
+    Lemma interp_lexps_instant_good:
+      forall es cks,
+        Forall (wt_lexp (idty vars)) es ->
+        Forall2 (wc_lexp (idck vars)) es cks ->
+        Forall Ops_defined_in_lexp es ->
+        var_inv (fun x => Exists (Is_free_in_lexp x) es) ->
+        exists vs, interp_lexps_instant es = Some vs.
+    Proof.
+      induction es as [|e es IH]. now exists [].
+      intros cks WTs WCs ODs Invs.
+      inversion_clear WTs as [|?? WT WTs'].
+      inversion_clear WCs as [|???? WC WCs'].
+      inversion_clear ODs as [|?? OD ODs'].
+      assert (var_inv (fun x=>Is_free_in_lexp x e)) as Inv
+          by (eapply var_inv_weaken; [eauto|now intuition]).
+      assert (var_inv (fun x=>Exists (Is_free_in_lexp x) es)) as Invs'
+          by (eapply (var_inv_weaken _ _ Invs); eauto).
+      simpl.
+      pose proof (interp_lexp_instant_good _ _ WT WC OD Inv) as (v & ->).
+      specialize (IH _ WTs' WCs' ODs' Invs') as (vs & ->).
+      eauto.
     Qed.
 
   End InstantInterpreter.
-
-  (** ** Liftings of instantaneous semantics *)
-
-  Section LiftInterpreter.
-
-    Variable bk : stream bool.
-    Variable H: history.
-
-    Definition lift {A B} (interp: bool -> env -> A -> B) x: stream B :=
-      fun n => interp (bk n) (restr_hist H n) x.
-
-    Definition lift' {A B} (interp: env -> A -> B) x: stream B :=
-      fun n => interp (restr_hist H n) x.
-
-    Definition interp_clock (ck: clock): stream bool :=
-      lift interp_clock_instant ck.
-
-    Definition interp_var (x: ident): stream value :=
-      lift' interp_var_instant x.
-
-    Definition interp_vars (xs: idents): stream (list value) :=
-      lift' interp_vars_instant xs.
-
-    Definition interp_lexp (e: lexp): stream value :=
-      lift interp_lexp_instant e.
-
-    Definition interp_lexps (e: list lexp): stream (list value) :=
-      lift interp_lexps_instant e.
-
-    Definition interp_lexps' (e: list lexp): list (stream value) :=
-      map interp_lexp e.
-
-    Lemma interp_lexps'_sound:
-      forall es ess,
-        sem_lexps bk H es ess ->
-        Forall2 (sem_lexp bk H) es (interp_lexps' es).
-    Proof.
-      induction es; intros * Sem; simpl; auto.
-      constructor.
-      - intro n; specialize (Sem n); inv Sem.
-        unfold interp_lexp, lift.
-        erewrite <-interp_lexp_instant_sound; eauto.
-      - eapply IHes.
-        intro n; specialize (Sem n); inv Sem.
-        instantiate (1 := fun n => tl (ess n)).
-        simpl.
-        rewrite <-H2; simpl; auto.
-    Qed.
-
-    Definition interp_cexp (e: cexp): stream value :=
-      lift interp_cexp_instant e.
-
-    Definition interp_caexp (ck: clock) (e: cexp): stream value :=
-      lift (fun base R => interp_caexp_instant base R ck) e.
-
-    Definition interp_laexp (ck: clock) (e: lexp): stream value :=
-      lift (fun base R => interp_laexp_instant base R ck) e.
-
-    Lemma lift_sound:
-      forall {A B} (sem: bool -> env -> A -> B -> Prop) interp x xs,
-        (forall b R x v, sem b R x v -> v = interp b R x) ->
-        CESem.lift bk H sem x xs ->
-        xs ≈ lift interp x.
-    Proof.
-      intros * Instant Sem n.
-      specialize (Sem n); unfold lift; auto.
-    Qed.
-
-    Lemma lift'_sound:
-      forall {A B} (sem: env -> A -> B -> Prop) interp x xs,
-        (forall R x v, sem R x v -> v = interp R x) ->
-        CESem.lift' H sem x xs ->
-        xs ≈ lift' interp x.
-    Proof.
-      intros * Instant Sem n.
-      specialize (Sem n); unfold lift'; auto.
-    Qed.
-
-    Corollary interp_clock_sound:
-      forall ck bs,
-        sem_clock bk H ck bs ->
-        bs ≈ interp_clock ck.
-    Proof.
-      intros; eapply lift_sound; eauto;
-        apply interp_clock_instant_sound.
-    Qed.
-
-    Corollary interp_var_sound:
-      forall x vs,
-        sem_var H x vs ->
-        vs ≈ interp_var x.
-    Proof.
-      intros; eapply lift'_sound; eauto;
-        apply interp_var_instant_sound.
-    Qed.
-
-    Corollary interp_vars_sound:
-      forall xs vss,
-        sem_vars H xs vss ->
-        vss ≈ interp_vars xs.
-    Proof.
-      intros; eapply lift'_sound; eauto;
-        apply interp_vars_instant_sound.
-    Qed.
-
-    Corollary interp_lexp_sound:
-      forall e vs,
-        sem_lexp bk H e vs ->
-        vs ≈ interp_lexp e.
-    Proof.
-      intros; eapply lift_sound; eauto;
-        apply interp_lexp_instant_sound.
-    Qed.
-
-    Corollary interp_lexps_sound:
-      forall es vss,
-        sem_lexps bk H es vss ->
-        vss ≈ interp_lexps es.
-    Proof.
-      intros; eapply lift_sound; eauto;
-        apply interp_lexps_instant_sound.
-    Qed.
-
-    Corollary interp_cexp_sound:
-      forall e vs,
-        sem_cexp bk H e vs ->
-        vs ≈ interp_cexp e.
-    Proof.
-      intros; eapply lift_sound; eauto;
-        apply interp_cexp_instant_sound.
-    Qed.
-
-    Corollary interp_laexp_sound:
-      forall e ck vs,
-        sem_laexp bk H ck e vs ->
-        vs ≈ interp_laexp ck e.
-    Proof.
-      intros; eapply lift_sound; eauto.
-      intros; apply interp_laexp_instant_sound; auto.
-    Qed.
-
-    Corollary interp_caexp_sound:
-      forall e ck vs,
-        sem_caexp bk H ck e vs ->
-        vs ≈ interp_caexp ck e.
-    Proof.
-      intros; eapply lift_sound; eauto.
-      intros; apply interp_caexp_instant_sound; auto.
-    Qed.
-    (* Definition interp_annotated {A} (interp_instant: bool -> env -> A -> value) (ck: clock) (a: A): stream value := *)
-    (*   lift (fun base R => interp_annotated_instant base R interp_instant ck) a. *)
-
-  End LiftInterpreter.
 
 End CEINTERPRETER.
 
@@ -399,7 +929,10 @@ Module CEInterpreterFun
        (Import CESyn : CESYNTAX        Op)
        (Import Str   : STREAM          Op OpAux)
        (Import CESem : CESEMANTICS Ids Op OpAux CESyn Str)
-       <: CEINTERPRETER Ids Op OpAux CESyn Str CESem.
-  Include CEINTERPRETER Ids Op OpAux CESyn Str CESem.
+       (Import CETyp : CETYPING    Ids Op       CESyn)
+       (Import CEClk : CECLOCKING  Ids Op       CESyn)
+       (Import CEFree: CEISFREE    Ids Op       CESyn)
+       <: CEINTERPRETER Ids Op OpAux CESyn Str CESem CETyp CEClk CEFree.
+  Include CEINTERPRETER Ids Op OpAux CESyn Str CESem CETyp CEClk CEFree.
 End CEInterpreterFun.
 
